Remodel nested inductive example to a verified Trie

Hashmap/Example/NestedInductiveSafe.lean
@@ -11,17 +11,6 @@ declare an inductive predicate for the well-formedness.
 
 open MyLean
 
-inductive RawTree where
-  | leaf : Nat → RawTree
-  | internal : HashMap.Raw Nat RawTree → RawTree
-
-def RawTree.child? (n : Nat) : RawTree → Option RawTree
-  | .leaf _ => none
-  | .internal m => m.find? n
-
-@[simp] theorem RawTree.child?_leaf {n m : Nat} : (RawTree.leaf n).child? m = none := rfl
-@[simp] theorem RawTree.child?_internal {m : HashMap.Raw Nat RawTree} {n : Nat} : (RawTree.internal m).child? n = m.find? n := rfl
-
 def hasValue [BEq α] [Hashable α] (m : HashMap.Raw α β) (b : β) : Prop :=
   ∃ a, m.find? a = some b
 
@@ -45,66 +34,181 @@ theorem hasValue_insert [BEq α] [Hashable α] [EquivBEq α] [LawfulHashable α]
     · exact ⟨a, by simp⟩
     · exact ⟨a', by simp_all⟩
 
-inductive RawTree.WF : RawTree → Prop where
-  | leaf {n} : (RawTree.leaf n).WF
-  | internal {m : HashMap.Raw Nat RawTree} :
-      m.WF → (∀ t, hasValue m t → t.WF) → (RawTree.internal m).WF
+instance : Hashable Char where
+  hash c := hash c.val
 
-theorem RawTree.WF.child? {r : RawTree} (h : r.WF) {n : Nat} {c : RawTree} (h₂ : r.child? n = some c) :
-    c.WF := by
-  cases r
-  · simp at h₂
-  · rcases h with _|⟨-, h⟩
-    exact h _ ⟨_, h₂⟩
+inductive RawTrie (α : Type u) where
+  | mk : Bool → HashMap.Raw α (RawTrie α) → RawTrie α
 
-def Tree := { r : RawTree // r.WF }
+namespace RawTrie
 
-def Tree.leaf (n : Nat) : Tree :=
-  ⟨.leaf n, .leaf⟩
+def contained : RawTrie α → Bool
+  | .mk b _ => b
 
--- I wonder how hard it would be to convince the compiler to
-def Tree.child (n : Nat) (t : Tree) : Option Tree :=
-  match h : t.1.child? n with
-  | some c => some ⟨c, t.2.child? h⟩
-  | none => none
+def children : RawTrie α → HashMap.Raw α (RawTrie α)
+  | .mk _ m => m
 
--- set_option trace.compiler.ir.result true in
-def Tree.traverse : Tree → List Nat → Option Nat
-  | ⟨RawTree.leaf n, _⟩, [] => n
-  | t@⟨RawTree.internal _, _⟩, (i :: is) => t.child i |>.bind (·.traverse is)
-  | _, _ => none
+@[simp] theorem contained_mk {b : Bool} {m : HashMap.Raw α (RawTrie α)} : (RawTrie.mk b m).contained = b := rfl
+@[simp] theorem children_mk {b : Bool} {m : HashMap.Raw α (RawTrie α)} : (RawTrie.mk b m).children = m := rfl
 
-inductive ListTree where
-  | leaf : Nat → ListTree
-  | internal : List (Nat × ListTree) → ListTree
+def child? [BEq α] [Hashable α] (a : α) (t : RawTrie α) : Option (RawTrie α) :=
+  t.children.find? a
 
-def ListTree.toRawTree : ListTree → RawTree
-  | .leaf n => .leaf n
-  | .internal l => .internal (go ∅ l)
-where go (acc : HashMap.Raw Nat RawTree) : List (Nat × ListTree) → HashMap.Raw Nat RawTree
-  | [] => acc
-  | ⟨n, c⟩::ls => go (acc.insert n c.toRawTree) ls
+def empty : RawTrie α :=
+  ⟨false, ∅⟩
+
+@[simp] theorem children_empty : (empty : RawTrie α).children = ∅ := rfl
+@[simp] theorem contained_empty : (empty : RawTrie α).contained = false := rfl
+
+@[simp] theorem child?_empty [BEq α] [Hashable α] [EquivBEq α] [LawfulHashable α] (a : α) : (empty : RawTrie α).child? a = none := by
+  simp [child?]
+
+instance : EmptyCollection (RawTrie α) where
+  emptyCollection := .empty
+
+@[simp] theorem children_emptyc : (∅ : RawTrie α).children = ∅ := rfl
+@[simp] theorem contained_emptyc : (∅ : RawTrie α).contained = false := rfl
+
+def child [BEq α] [Hashable α] (a : α) (t : RawTrie α) : RawTrie α :=
+  (t.child? a).getD ∅
+
+def contains [BEq α] [Hashable α] : List α → RawTrie α → Bool
+  | [], t => t.contained
+  | (a::as), t => match t.child? a with
+    | none => false
+    | some u => u.contains as
 
 @[simp]
-theorem ListTree.toRawTree_leaf {n : Nat} : (ListTree.leaf n).toRawTree = RawTree.leaf n := by
-  rw [ListTree.toRawTree]
+theorem contains_nil_mk [BEq α] [Hashable α] {b : Bool} {m : HashMap.Raw α (RawTrie α)} :
+    (RawTrie.mk b m).contains [] = b := rfl
 
-theorem ListTree.WF_toRawTree (l : ListTree) : l.toRawTree.WF := by
-  suffices (∀ (acc : HashMap.Raw Nat RawTree) (l : List (Nat × ListTree)), acc.WF → (∀ t, hasValue acc t → t.WF) →
-    (toRawTree.go acc l).WF ∧ (∀ t, hasValue (toRawTree.go acc l) t → t.WF)) ∧ (∀ l, (ListTree.toRawTree l).WF) from this.2 _
-  apply toRawTree.go.mutual_induct
-  · intros acc h h'
-    refine ⟨?_, ?_⟩ <;> rwa [toRawTree.go]
-  · intros acc n c ls hc hins hacc hacc'
-    rw [toRawTree.go]
-    refine hins hacc.insert fun t h => ((hasValue_insert hacc).1 h).elim (· ▸ hc) ?_
-    rintro ⟨a', -, ha'⟩
-    exact hacc' _ ⟨a', ha'⟩
-  · simpa using fun _ => .leaf
-  · intro l h
-    rw [ListTree.toRawTree]
-    have := h HashMap.Raw.WF.empty (by simp)
-    exact .internal this.1 this.2
+def insert [BEq α] [Hashable α] : List α → RawTrie α → RawTrie α
+  | [], t => ⟨true, t.children⟩
+  | (a::as), t => ⟨t.contained, t.children.insert a ((t.child a).insert as)⟩
 
-def ListTree.toTree (t : ListTree) : Tree :=
-  ⟨t.toRawTree, WF_toRawTree t⟩
+inductive WF [BEq α] [Hashable α] : RawTrie α → Prop where
+  | mk {t : RawTrie α} : t.children.WF → (∀ c [EquivBEq α] [LawfulHashable α], hasValue t.children c → c.WF) → t.WF
+
+theorem WF.WF_children [BEq α] [Hashable α] {t : RawTrie α} : t.WF → t.children.WF
+  | ⟨h, _⟩ => h
+
+theorem WF.WF_of_hasValue [BEq α] [Hashable α] [EquivBEq α] [LawfulHashable α] {t : RawTrie α} : t.WF → ∀ c, hasValue t.children c → c.WF
+  | ⟨_, h⟩ => fun c => h c
+
+@[simp]
+theorem WF.empty [BEq α] [Hashable α] : (RawTrie.empty : RawTrie α).WF :=
+  ⟨by simpa using HashMap.Raw.WF.emptyc, fun _ _ _ => by simp⟩
+
+@[simp]
+theorem WF.emptyc [BEq α] [Hashable α] : (∅ : RawTrie α).WF :=
+  WF.empty
+
+theorem WF.child? [BEq α] [Hashable α] [EquivBEq α] [LawfulHashable α] {r : RawTrie α} (h : r.WF) {c : α} {s : RawTrie α} (h₂ : r.child? c = some s) :
+    s.WF := by
+  rcases h with ⟨-, h⟩
+  exact h _ ⟨_, h₂⟩
+
+theorem WF.child [BEq α] [Hashable α] [EquivBEq α] [LawfulHashable α] {r : RawTrie α} (h : r.WF) {c : α} : (r.child c).WF := by
+  rw [RawTrie.child]
+  cases hc : RawTrie.child? c r
+  · simp
+  · simpa using WF.child? h hc
+
+theorem WF.insert [BEq α] [Hashable α] {l : List α} {t : RawTrie α} (h : t.WF) : (t.insert l).WF := by
+  induction l, t using insert.induct
+  · rw [RawTrie.insert]
+    exact ⟨by simpa using h.WF_children, fun _ _ _ => by simpa using h.WF_of_hasValue _⟩
+  · next a as u ih =>
+    rw [RawTrie.insert]
+    refine ⟨h.WF_children.insert, fun v _ _ hv => ((hasValue_insert h.WF_children).1 hv).elim ?_ ?_⟩
+    · exact fun hx => hx ▸ ih h.child
+    · rintro ⟨a', -, ha'₂⟩
+      exact h.WF_of_hasValue _ ⟨a', ha'₂⟩
+
+@[simp]
+theorem contains_empty [BEq α] [Hashable α] [EquivBEq α] [LawfulHashable α] {l : List α} :
+    (RawTrie.empty : RawTrie α).contains l = false := by
+  induction l <;> simp [contains]
+
+@[simp]
+theorem contains_emptyc [BEq α] [Hashable α] [EquivBEq α] [LawfulHashable α] {l : List α} :
+    (∅ : RawTrie α).contains l = false :=
+  contains_empty
+
+example [BEq α] : BEq (List α) := by exact inferInstance
+
+theorem contains_insert [BEq α] [Hashable α] [EquivBEq α] [LawfulHashable α] {l m : List α} {t : RawTrie α} (h : t.WF) :
+    (t.insert l).contains m = ((l == m) || t.contains m) := by
+  induction l, t using insert.induct generalizing m
+  · rw [insert]
+    cases m
+    · simp only [contains_nil_mk, Bool.cond_true_left, Bool.true_eq, Bool.or_eq_true]
+      exact Or.inl rfl
+    · next a as =>
+      have : ([] == (a :: as)) = false := rfl
+      rw [contains, contains, this, Bool.false_or]
+      congr
+  · next a as u ih =>
+    rw [insert]
+    cases m
+    · have : ((a :: as) == []) = false := rfl
+      rw [contains_nil_mk, this, Bool.false_or, contains]
+    · next b bs =>
+      rw [contains, child?, children_mk, HashMap.Raw.find?_insert _ h.WF_children]
+      cases hab : a == b
+      · rw [cond_false]
+        have : (a :: as == b :: bs) = false := by
+          change (a == b && _) = false -- TODO: BEq List lemmas
+          rw [hab, Bool.false_and]
+        rw [this, Bool.false_or, contains]
+        rfl
+      · rw [cond_true]
+        dsimp only
+        rw [ih h.child]
+        have : (a :: as == b :: bs) = (as == bs) := by
+          change (a == b && _) = (as == bs)
+          rw [hab, Bool.true_and]
+          rfl
+        rw [this]
+        congr 1
+        rw [contains, child]
+        have hch : child? a u = child? b u := by
+          rw [child?, child?, HashMap.Raw.find?_congr _ h.WF_children hab]
+        rw [hch]
+        cases child? b u
+        · rw [Option.getD_none, contains_emptyc]
+        · rw [Option.getD_some]
+
+end RawTrie
+
+def Trie (α : Type u) [BEq α] [Hashable α] := { r : RawTrie α // r.WF }
+
+namespace Trie
+
+def empty [BEq α] [Hashable α] : Trie α :=
+  ⟨RawTrie.empty, RawTrie.WF.empty⟩
+
+instance [BEq α] [Hashable α] : EmptyCollection (Trie α) where
+  emptyCollection := .empty
+
+def insert [BEq α] [Hashable α] (l : List α) (t : Trie α) : Trie α :=
+  ⟨t.1.insert l, t.2.insert⟩
+
+def contains [BEq α] [Hashable α] (l : List α) (t : Trie α) : Bool :=
+  t.1.contains l
+
+@[simp]
+theorem contains_empty [BEq α] [Hashable α] [EquivBEq α] [LawfulHashable α] {l : List α} :
+    (Trie.empty : Trie α).contains l = false :=
+  RawTrie.contains_empty
+
+@[simp]
+theorem contains_emptyc [BEq α] [Hashable α] [EquivBEq α] [LawfulHashable α] {l : List α} :
+    (∅ : Trie α).contains l = false :=
+  RawTrie.contains_emptyc
+
+theorem contains_insert [BEq α] [Hashable α] [EquivBEq α] [LawfulHashable α] {l m : List α} {t : Trie α} :
+    (t.insert l).contains m = ((l == m) || t.contains m) :=
+  RawTrie.contains_insert t.2
+
+end Trie
