Hashmap/HashMap/Lemmas.lean
@@ -45,6 +45,9 @@ theorem find?_insert {a k : α} {b : β} :
     (m.insert a b).find? k = bif a == k then some b else m.find? k := by
   simp [find?, insert, DHashMap.Raw.findConst?_insert _ h]
 
+theorem find?_congr {a b : α} (hab : a == b) : m.find? a = m.find? b := by
+  simp [find?, DHashMap.Raw.findConst?_congr _ h hab]
+
 end Raw
 
 section
